Soundness

theories/AL/AL.v
@@ -1,5 +1,5 @@
 From Stdlib Require Export NArith String.
-From ILAL Require Export AL.language state.
+From ILAL Require Export AL.language state tactics.
 From Stdlib Require Import List.
 Import ListNotations.
 Open Scope N_scope.
@@ -21,9 +21,40 @@ Reserved Notation
    m constr, s constr, s' constr).
 
 Open Scope al_scope.
+
+Definition mode_store (m : mode) (sig : estate) : state :=
+  match m with
+  | Ok => sig.(vstate).(s)
+  | Ad => sig.(astate).(s)
+  end.
+
+(* Mode-aware update *)
+Definition mode_upd (m : mode) (sig : estate) (x : id) (v : N) : estate :=
+  match m with
+  | Ok => sig[[ x :=v v ]]
+  | Ad => sig[[ x :=a v ]]
+  end.
+
+(* Channel [k]'s contents in [m]'s store *)
+Definition mode_chan (m : mode) (sig : estate) (k : id) : channel :=
+  match m with
+  | Ok => sig.(vstate).(ch) k
+  | Ad => sig.(astate).(ch) k
+  end.
+
+(* [k] :=m [l] *)
+Definition mode_chan_upd (m : mode) (sig : estate) (k : id) (l : channel) : estate :=
+  match m with
+  | Ok => sig[[ k :=vch l ]]
+  | Ad => sig[[ k :=ach l ]]
+  end.
+
 Inductive ds : astmt -> mode -> (estate * estate) -> Prop :=
 | EDSkip m (s : estate) :
     [[ skip ]] m |=> (s, s)
+| EDAssume (B : prop) m (sig : estate) :
+    B (mode_store m sig) ->
+    [[ assume(B) ]] m |=> (sig, sig)
 | EDAssignV x e (st : estate) :
     [[ x := e ]] Ok |=> (st, st[[ x :=v e (st.(vstate).(s)) ]])
 | EDAssignA x e (st : estate) :
@@ -46,10 +77,10 @@ Inductive ds : astmt -> mode -> (estate * estate) -> Prop :=
 (** write(s, x): append var x to channel s *)
 | EDWriteV (ch_id x : id) (sig : estate) :
     [[ write(ch_id, x) ]] Ok |=>
-      (sig, sig[[ ch_id :=vch sig.(vstate).(s) x :: sig.(vstate).(ch) ch_id ]])
+      (sig, sig[[ ch_id :=vch (sig.(vstate).(ch) ch_id ++ [sig.(vstate).(s) x]) ]])%list
 | EDWriteA (ch_id x : id) (sig : estate) :
     [[ write(ch_id, x) ]] Ad |=>
-      (sig, sig[[ ch_id :=ach sig.(astate).(s) x :: sig.(astate).(ch) ch_id ]])
+      (sig, sig[[ ch_id :=ach (sig.(astate).(ch) ch_id ++ [sig.(astate).(s) x]) ]])%list
 (** adv_assert(P): adversarial assert *)
 | EDAdvAssertSuccess P (sig : estate) :
     P sig.(astate).(s) ->
@@ -57,6 +88,20 @@ Inductive ds : astmt -> mode -> (estate * estate) -> Prop :=
 | EDAdvAssertFailure P (sig : estate) :
     ~ P sig.(astate).(s) ->
     [[ adv_assert(P) ]] Ad |=> (sig, sig)
+(** C1 + C2: nondeterministic choice *)
+| EDChoiceL c1 c2 m s1 s2 :
+    [[ c1 ]] m |=> (s1, s2) ->
+    [[ c1 <+> c2 ]] m |=> (s1, s2)
+| EDChoiceR c1 c2 m s1 s2 :
+    [[ c2 ]] m |=> (s1, s2) ->
+    [[ c1 <+> c2 ]] m |=> (s1, s2)
+(** C*: Kleene iteration *)
+| EDStar0 c m (s : estate) :
+    [[ c** ]] m |=> (s, s)
+| EDStarN c m s1 s2 s3 :
+    [[ c** ]] m |=> (s1, s2) ->
+    [[ c ]] m |=> (s2, s3) ->
+    [[ c** ]] m |=> (s1, s3)
 (** c1 || c2 *)
 | EDParL c1 c2 m s1 s2 :
     [[ c1 ]] m |=> (s1, s2) ->
@@ -91,9 +136,26 @@ Definition over_approximate (P : aprop) (c : astmt) (m : mode) (Q : aprop) : Pro
 
 Notation "<| P |> c [[ m ]] <| Q |>" :=
   (over_approximate P c m Q)
-  (at level 90, c custom al_stmt at level 99, m constr) : al_scope.
+  (at level 0, c custom al_stmt at level 99, m constr) : al_scope.
 
-(* Definition 2 *)
+(** Lifting predicates into adversarial predicates  *)
+Definition lift (m : mode) (B : prop) : aprop :=
+  fun sig => B (mode_store m sig).
+
+Definition aand (P : aprop) (Q : aprop) : aprop :=
+  fun sig => P sig /\ Q sig.
+
+Definition aor (P : aprop) (Q : aprop) : aprop :=
+  fun sig => P sig \/ Q sig.
+
+Definition anot (P : aprop) : aprop :=
+  fun sig => ~ P sig.
+
+(* [P /\ B[m]] *)
+Definition aand_lift (m : mode) (P : aprop) (B : prop) : aprop :=
+  aand P (lift m B).
+
+(** Definition 2 *)
 
 Definition aprop2 : Type := estate -> estate -> Prop.
 
@@ -109,23 +171,19 @@ Definition al_under2 (P A : aprop) (c1 c2 : astmt) (Q B : aprop) : Prop :=
 
 Notation "<[[ P ]][[ A ]] c1 || c2 [[ Q ]][[ B ]]>" :=
   (al_under2 P A c1 c2 Q B)
-  (at level 90, c1 custom al_stmt at level 99, c2 custom al_stmt at level 99) : al_scope.
+  (at level 0, c1 custom al_stmt at level 99, c2 custom al_stmt at level 99) : al_scope.
 
 Open Scope al_scope.
 
-(* Definition 3 *)
+(** Definition 3 *)
 
 Theorem and_or_symmetry : forall P Q1 Q2 c m,
   ({{ P }} c [[m]] {{ Q1 }} /\ {{ P }} c [[m]] {{ Q2 }}) <->
   {{ P }} c [[m]] {{ fun s => Q1 s \/ Q2 s }}.
 Proof.
-  intros. split; intro H.
-  - destruct H as [H1 H2]. intros s [HQ1 | HQ2].
-    + apply H1, HQ1.
-    + apply H2, HQ2.
-  - split; intros s Hs.
-    + apply H. now left.
-    + apply H. now right.
+  intros. split; intros.
+  - destruct H as [H1 H2]. intros s [HQ1 | HQ2]; auto.
+  - split; intros s Hs; auto.
 Qed.
 
 Theorem impl_symmetry : forall P P' Q Q' c m,
@@ -149,9 +207,7 @@ Proof.
   intros u u' c m o o' HU HUO HO s Hu's.
   apply HO.
   destruct (HU s Hu's) as (s' & Hs' & Step).
-  exists s'. split.
-    apply HUO, Hs'.
-    assumption.
+  exists s'. auto.
 Qed.
 
 Theorem al_principle_of_denial : forall u u' c m o o',
@@ -163,83 +219,10 @@ Proof.
   intros u u' c m o o' HU HUO HNO HO.
   apply HNO. intros s Hu's.
   destruct (HU s Hu's) as (s' & Hs' & Step).
-  eapply HO. exists s'. split.
-    apply HUO, Hs'.
-    assumption.
+  eapply HO. exists s'. auto.
 Qed.
 
-Reserved Notation
-  "P , [[ c ]] m , Q"
-  (at level 40, c custom al_stmt at level 99).
-Inductive derivable: aprop -> astmt -> mode -> aprop -> Prop :=
-| Unit P m:
-  P, [[skip]] m, P
-| Consequence P P' Q Q' c m :
-  P, [[c]] m, Q ->
-  P ->> P' ->
-  Q' ->> Q ->
-  P', [[c]] m, Q'
-(**  Not sure if assume should be B sig or B sig.(a/vstate).(s)**)
-| AssumeOk P B :
-  P, [[assume(B)]] Ok, (fun sig => P sig /\ B sig.(vstate).(s))
-| AssumeAd P B :
-  P, [[assume(B)]] Ad, (fun sig => P sig /\ B sig.(astate).(s))
-| Disjunction P1 Q1 P2 Q2 c m :
-  P1, [[c]] m, Q1 ->
-  P2, [[c]] m, Q2 ->
-  (fun s => P1 s \/ P2 s), [[c]] m, (fun s => Q1 s \/ Q2 s)
-| Seq P Q R c1 c2 m :
-  P, [[c1]] m, Q -> 
-  Q, [[c2]] m, R ->
-  P, [[c1 ;; c2]] m, R
-| ChoiceLeft P Q c1 c2 m:
-  P, [[c1]] m, Q ->
-  P, [[c1 <+> c2]] m, Q
-| ChoiceRight P Q c1 c2 m:
-  P, [[c2]] m, Q ->
-  P, [[c1 <+> c2]] m, Q
-| IterateZero P c m:
-  P, [[c**]] m, P
-| IterateNonzero P Q c m :
-  P, [[c** ;; c]] m, Q ->
-  P, [[c**]] m, Q
-| LocalOk P x (e : expression):
-  P, [[x := e]] Ok, (fun sig => exists x', P (sig[[x :=v x' (sig.(vstate).(s))]]) /\ (sig.(vstate).(s) x) = e (sig[[x :=v x' (sig.(vstate).(s))]]).(vstate).(s))
-| LocalAd P x (e : expression):
-  P, [[x := e]] Ad, (fun sig => exists x', P (sig[[x :=a x' (sig.(astate).(s))]]) /\ (sig.(astate).(s) x) = e (sig[[x :=a x' (sig.(astate).(s))]]).(astate).(s))
-| ReadV P (ss x : id):
-  P, [[ read(ss, x) ]] Ok, (fun sig => exists (v : N) x' s', P ((sig[[x :=v x' (sig.(vstate).(s))]]) [[ss :=vch s' (sig.(vstate).(ch))]])
-                                                            /\ s' (sig.(vstate).(ch)) = v :: sig.(vstate).(ch) ss
-                                                            /\ sig.(vstate).(s) x = v)
-| ReadA P (ss x : id):
-  P, [[ read(ss, x) ]] Ad, (fun sig => exists (v : N) x' s', P ((sig[[x :=a x' (sig.(astate).(s))]]) [[ss :=ach s' (sig.(astate).(ch))]])
-                                                            /\ s' (sig.(astate).(ch)) = v :: sig.(astate).(ch) ss
-                                                            /\ sig.(astate).(s) x = v)
-| WriteV P (ss x : id):
-  P, [[ write(ss, x) ]] Ok, (fun sig => exists (v : N) s', P (sig[[ss :=vch s' (sig.(vstate).(ch))]])
-                                                          /\ sig.(vstate).(ch) ss = v :: s' (sig.(vstate).(ch))
-                                                          /\ sig.(vstate).(s) x = v)
-| WriteA P (ss x : id):
-  P, [[ write(ss, x) ]] Ok, (fun sig => exists (v : N) s', P (sig[[ss :=ach s' (sig.(astate).(ch))]])
-                                                          /\ sig.(astate).(ch) ss = v :: s' (sig.(astate).(ch))
-                                                          /\ sig.(astate).(s) x = v)
-| ParL P1 c1 Q1 P2 c2 Q2 m1 m2:
-  P1, [[c1]] m1, Q1 ->
-  P2, [[c2]] m2, Q2 ->
-  P1, [[c1 <||> c2]] m1, Q1 
-| ParR P1 c1 Q1 P2 c2 Q2 m1 m2:
-  P1, [[c1]] m1, Q1 ->
-  P2, [[c2]] m2, Q2 ->
-  P2, [[c1 <||> c2]] m2, Q2 
-(** I think this is the literal interpretation from the paper (for ok->ad and ad->ok only) as [P][A] c1 || c2 [Q][B] is defined as [P] c1 || c2 [Q] /\ [A] c1 || c2 [B] **)
-| ComVA_V P c1 A c2 (ss : id):
-  P, [[c1 <||> c2]] Ok, (fun sig => exists v s', (P (sig[[ss :=vch s' (sig.(vstate).(ch))]]) /\ s' (sig.(vstate).(ch)) = v :: sig.(vstate).(ch) ss /\ A (sig[[ss :=ach s' (sig.(astate).(ch))]]) /\ sig.(astate).(ch) ss = v :: s' (sig.(astate).(ch))))
-
-
-
-  
-where "P , [[ c ]] m , Q" := (derivable P c m Q).
-(* Lemma 1 *)
+(** Lemma 1 *)
 
 Lemma characterization :
   forall P Q A B C1 C2,
@@ -250,10 +233,336 @@ Lemma characterization :
 Proof.
   intros. unfold al_under2, al_post2. split; intro; intros.
   - specialize (H _ _ (conj H0 H1)). destruct H as (sq' & sb' & HQ & HB & DS1 & DS2).
-    exists sq', sb'. now repeat split.
+    exists sq', sb'. auto.
   - destruct H0. specialize (H _ _ H0 H1). destruct H as (sq' & sb' & HQ & HB & DS1 & DS2).
-    exists sq', sb'. now repeat split.
+    exists sq', sb'. auto.
 Qed.
 
 (** Proof rules *)
 (* Page 9 *)
+
+Reserved Notation
+         "P , [ c ] m , Q"
+         (at level 40, c custom al_stmt at level 99, P constr, Q constr).
+Inductive derivable : aprop -> astmt -> mode -> aprop -> Prop :=
+(* The empty postcondition is always under-approximate *)
+| DEmpty : forall P c m,
+    P, [c] m, (fun _ => False)
+(* Unit *)
+| DUnit : forall m P,
+    P, [skip] m, P
+(* Consequence *)
+| DConsequence : forall P P' Q Q' c m
+    (L: P ->> P')
+    (R: Q' ->> Q)
+    (Cons: P, [c] m, Q),
+    P', [c] m, Q'
+(* Disjunction *)
+| DDisj : forall P1 Q1 P2 Q2 c m,
+    P1, [c] m, Q1 ->
+    P2, [c] m, Q2 ->
+    (aor P1 P2), [c] m, (aor Q1 Q2)
+(* Sequencing *)
+| DSeq : forall P Q R c1 c2 m,
+    P, [c1] m, Q ->
+    Q, [c2] m, R ->
+    P, [c1 ;; c2] m, R
+(* Choice *)
+| DChoiceL : forall P Q c1 c2 m,
+    P, [c1] m, Q ->
+    P, [c1 <+> c2] m, Q
+| DChoiceR : forall P Q c1 c2 m,
+    P, [c2] m, Q ->
+    P, [c1 <+> c2] m, Q
+(* Iterate Zero *)
+| DIterZero : forall P c m,
+    P, [c**] m, P
+(* Iterate non-zero *)
+| DIterNonzero : forall P Q c m,
+    P, [c** ;; c] m, Q ->
+    P, [c**] m, Q
+(* Backward variant: a varying invariant [P n] preserved by one
+   iteration witnesses the iterated postcondition [exists n, P n] *)
+| DBackwardVariant : forall (P : nat -> aprop) c m,
+    (forall n, (P n), [c] m, (P (S n))) ->
+    (P O), [c**] m, (fun sig => exists n, P n sig)
+(* Assume: [eps: P] assume(B) [eps: P /\ B] *)
+| DAssume : forall P B m,
+    P, [assume(B)] m, (aand_lift m P B)
+(* Assignment *)
+| DAssign : forall P x (e : expression) m,
+    P, [x := e] m,
+       (fun sig => exists x', P (mode_upd m sig x x') /\
+                   mode_store m sig x = e (mode_store m (mode_upd m sig x x')))
+(* Rand *)
+| DRand : forall P x m,
+    P, [x := rand()] m,
+       (fun sig => exists x', P (mode_upd m sig x x'))
+(* Read(s,x): consume the head [v] of channel [s] into [x] *)
+| DRead : forall P (s x : id) m,
+    P, [read(s, x)] m,
+       (fun sig => exists v x' l,
+            P (mode_chan_upd m (mode_upd m sig x x') s (v :: l))
+            /\ mode_chan m sig s = l
+            /\ mode_store m sig x = v)
+(* Write(s,x): append the value of [x] to the end of channel [s] *)
+| DWrite : forall P (s x : id) m,
+    P, [write(s, x)] m,
+       (fun sig => exists l,
+            P (mode_chan_upd m sig s l)
+            /\ mode_chan m sig s = l ++ [mode_store m sig x])%list
+(* Adversarial assertion, success branch *)
+| DAdvAssertSuccess : forall Q B,
+    Q, [adv_assert(B)] Ad, (aand_lift Ad Q B)
+(* Adversarial assertion, failure branch *)
+| DAdvAssertFailure : forall Q B,
+    Q, [adv_assert(B)] Ad, (aand Q (anot (lift Ad B)))
+where "P , [ c ] m , Q" := (derivable P c m Q).
+
+Definition denote (c : astmt) (m : mode) : evaluation :=
+  fun '(s1, s2) => [[ c ]] m |=> (s1, s2).
+
+Definition interpret_spec (P Q : aprop) (c : astmt) m : Prop :=
+  P, [c] m, Q <-> {{P}} c [[m]] {{Q}}.
+
+Fixpoint nRepeat (c : astmt) (n : nat) : astmt :=
+  match n with
+  | O => ASkip
+  | S n' => ASeq (nRepeat c n') c
+  end.
+
+Lemma star_equiv : forall c m s1 s2,
+  [[ c** ;; c ]] m |=> (s1, s2) ->
+  [[ c** ]] m |=> (s1, s2).
+Proof.
+  intros c m s1 s2 H. invs H. econstructor; eassumption.
+Qed.
+
+Lemma nRepeat_star : forall c m n s1 s2,
+  ds (nRepeat c n) m (s1, s2) ->
+  [[ c** ]] m |=> (s1, s2).
+Proof.
+  intros c m n. induction n; intros s1 s2 H.
+  - simpl in H. invs H. constructor.
+  - simpl in H. invs H. econstructor; eauto.
+Qed.
+
+(* Conversely, every star execution is some finite [n]-fold repetition *)
+Lemma star_nRepeat : forall c m s1 s2,
+  [[ c** ]] m |=> (s1, s2) ->
+  exists n, ds (nRepeat c n) m (s1, s2).
+Proof.
+  intros c m s1 s2 H.
+  remember <{ c** }> as cs eqn:E.
+  induction H; invs E.
+  - exists O. constructor.
+  - destruct (IHds1 eq_refl) as (n & Hn).
+    exists (S n). econstructor; eauto.
+Qed.
+
+Lemma repeat_is_star : forall c m P s,
+  post (denote <{ c** }> m) P s ->
+  exists n, post (denote (nRepeat c n) m) P s.
+Proof.
+  intros c m P s (s' & Ps' & DS). unfold denote in DS.
+  apply star_nRepeat in DS. destruct DS as (n & Hn).
+  exists n, s'. now split.
+Qed.
+
+Lemma step_assign_ok : forall sig x (e : expression) x',
+  sig.(vstate).(s) x = e ((sig[[ x :=v x' ]]).(vstate).(s)) ->
+  [[ x := e ]] Ok |=> (sig[[ x :=v x' ]], sig).
+Proof.
+  intros [(vs & vc) (as_  & ac)] x e x' Eq. simpl in *.
+  replace ({| vstate := {| s := vs; ch := vc |};
+              astate := {| s := as_; ch := ac |} |})
+    with ((({| vstate := {| s := vs; ch := vc |};
+               astate := {| s := as_; ch := ac |} |})[[ x :=v x' ]])
+            [[ x :=v e (({| vstate := {| s := vs; ch := vc |};
+                           astate := {| s := as_; ch := ac |} |})[[ x :=v x' ]]).(vstate).(s) ]])
+    at 2.
+    apply EDAssignV.
+  unfold update_victim. simpl. f_equal. f_equal.
+  now rewrite update_shadow, <- Eq, state_upd_eq.
+Qed.
+
+Lemma step_assign_ad : forall sig x (e : expression) x',
+  sig.(astate).(s) x = e ((sig[[ x :=a x' ]]).(astate).(s)) ->
+  [[ x := e ]] Ad |=> (sig[[ x :=a x' ]], sig).
+Proof.
+  intros [(vs & vc) (as_  & ac)] x e x' Eq. simpl in *.
+  replace ({| vstate := {| s := vs; ch := vc |};
+              astate := {| s := as_; ch := ac |} |})
+    with ((({| vstate := {| s := vs; ch := vc |};
+               astate := {| s := as_; ch := ac |} |})[[ x :=a x' ]])
+            [[ x :=a e (({| vstate := {| s := vs; ch := vc |};
+                           astate := {| s := as_; ch := ac |} |})[[ x :=a x' ]]).(astate).(s) ]])
+    at 2.
+    apply EDAssignA.
+  unfold update_adversary. simpl. f_equal. f_equal.
+  now rewrite update_shadow, <- Eq, state_upd_eq.
+Qed.
+
+Lemma step_rand_ok : forall sig x x',
+  [[ x := rand() ]] Ok |=> (sig[[ x :=v x' ]], sig).
+Proof.
+  intros [(vs & vc) (as_ & ac)] x x'.
+  assert (E : (({| vstate := {| s := vs; ch := vc |};
+                   astate := {| s := as_; ch := ac |} |})[[ x :=v x' ]])
+                [[ x :=v vs x ]]
+              = {| vstate := {| s := vs; ch := vc |};
+                   astate := {| s := as_; ch := ac |} |}).
+  { unfold update_victim. simpl. f_equal. f_equal.
+    now rewrite update_shadow, state_upd_eq. }
+  rewrite <- E at 2. apply EDRandV.
+Qed.
+ 
+Lemma step_rand_ad : forall sig x x',
+  [[ x := rand() ]] Ad |=> (sig[[ x :=a x' ]], sig).
+Proof.
+  intros [(vs & vc) (as_ & ac)] x x'.
+  assert (E : (({| vstate := {| s := vs; ch := vc |};
+                   astate := {| s := as_; ch := ac |} |})[[ x :=a x' ]])
+                [[ x :=a as_ x ]]
+              = {| vstate := {| s := vs; ch := vc |};
+                   astate := {| s := as_; ch := ac |} |}).
+  { unfold update_adversary. simpl. f_equal. f_equal.
+    now rewrite update_shadow, state_upd_eq. }
+  rewrite <- E at 2. apply EDRandA.
+Qed.
+
+Lemma step_read_ok : forall sig (s_ x : id) v x' l,
+  sig.(vstate).(ch) s_ = l ->
+  sig.(vstate).(s) x = v ->
+  [[ read(s_, x) ]] Ok |=> ((sig[[ x :=v x' ]])[[ s_ :=vch v :: l ]], sig).
+Proof.
+  intros [(vs & vc) (as_ & ac)] s x v x' l Hl Hx. simpl in *.
+  replace ({| vstate := {| s := vs; ch := vc |};
+              astate := {| s := as_; ch := ac |} |})
+    with ((((({| vstate := {| s := vs; ch := vc |};
+                 astate := {| s := as_; ch := ac |} |})[[ x :=v x' ]])
+              [[ s :=vch v :: l ]])[[ x :=v v ]])[[ s :=vch l ]])
+    at 2.
+  - apply EDReadV. unfold update_vchannel, update_victim.
+    simpl. now rewrite update_eq.
+  - unfold update_vchannel, update_victim. simpl. f_equal.
+    f_equal; rewrite update_shadow.
+    now rewrite <- Hx, state_upd_eq.
+    now rewrite <- Hl, state_upd_eq.
+Qed.
+
+Lemma step_read_ad : forall sig (s_ x : id) v x' l,
+  sig.(astate).(ch) s_ = l ->
+  sig.(astate).(s) x = v ->
+  [[ read(s_, x) ]] Ad |=> ((sig[[ x :=a x' ]])[[ s_ :=ach v :: l ]], sig).
+Proof.
+  intros [(vs & vc) (as_ & ac)] s x v x' l Hl Hx. simpl in *.
+  replace ({| vstate := {| s := vs; ch := vc |};
+              astate := {| s := as_; ch := ac |} |})
+    with ((((({| vstate := {| s := vs; ch := vc |};
+                 astate := {| s := as_; ch := ac |} |})[[ x :=a x' ]])
+              [[ s :=ach v :: l ]])[[ x :=a v ]])[[ s :=ach l ]])
+    at 2.
+  - apply EDReadA. unfold update_achannel, update_adversary.
+    simpl. now rewrite update_eq.
+  - unfold update_achannel, update_adversary. simpl. f_equal.
+    f_equal; rewrite update_shadow.
+    now rewrite <- Hx, state_upd_eq.
+    now rewrite <- Hl, state_upd_eq.
+Qed.
+
+Lemma step_write_ok : forall sig (s_ x : id) l,
+  sig.(vstate).(ch) s_ = (l ++ [sig.(vstate).(s) x])%list ->
+  [[ write(s_, x) ]] Ok |=> (sig[[ s_ :=vch l ]], sig).
+Proof.
+  intros [(vs & vc) (as_ & ac)] s x l Hl. simpl in *.
+  assert (E : ({| vstate := {| s := vs; ch := vc |};
+                  astate := {| s := as_; ch := ac |} |})
+              = (({| vstate := {| s := vs; ch := update vc s l |};
+                     astate := {| s := as_; ch := ac |} |})
+                 [[ s :=vch ((update vc s l) s ++ [vs x]) ]])%list).
+  { unfold update_vchannel. simpl. rewrite update_eq.
+    f_equal. f_equal. now rewrite update_shadow, <- Hl, state_upd_eq. }
+  unfold update_vchannel. simpl. rewrite E. apply EDWriteV.
+Qed.
+
+Lemma step_write_ad : forall sig (s_ x : id) l,
+  sig.(astate).(ch) s_ = (l ++ [sig.(astate).(s) x])%list ->
+  [[ write(s_, x) ]] Ad |=> (sig[[ s_ :=ach l ]], sig).
+Proof.
+  intros [(vs & vc) (as_ & ac)] s x l Hl. simpl in *.
+  assert (E : ({| vstate := {| s := vs; ch := vc |};
+                  astate := {| s := as_; ch := ac |} |})
+              = (({| vstate := {| s := vs; ch := vc |};
+                     astate := {| s := as_; ch := (update ac s l) |} |})
+                 [[ s :=ach ((update ac s l) s ++ [as_ x]) ]])%list).
+  { unfold update_achannel. simpl. rewrite update_eq.
+    f_equal. f_equal. now rewrite update_shadow, <- Hl, state_upd_eq. }
+  unfold update_achannel. simpl. rewrite E. apply EDWriteA.
+Qed.
+
+Theorem soundness :
+  forall c P Q m,
+    P, [c] m, Q ->
+    {{P}} c [[m]] {{Q}}.
+Proof.
+  intros c P Q m H. induction H.
+  - (* DEmpty *) intros s Fs. contradiction.
+  - (* DUnit *) intros s Ps. exists s. split. assumption. constructor.
+  - (* DConsequence *) intros s Q's. apply R in Q's.
+    destruct (IHderivable s Q's) as (s' & Qs' & DS).
+    exists s'. auto.
+  - (* DDisj *) intros s [Q1s | Q2s].
+    + destruct (IHderivable1 s Q1s) as (s' & P1s' & DS).
+      exists s'. split. now left. assumption.
+    + destruct (IHderivable2 s Q2s) as (s' & P2s' & DS).
+      exists s'. split. now right. assumption.
+  - (* DSeq *) intros s Rs.
+    destruct (IHderivable2 s Rs) as (s2 & Qs2 & DS2).
+    destruct (IHderivable1 s2 Qs2) as (s1 & Ps1 & DS1).
+    exists s1. split. assumption. econstructor; eassumption.
+  - (* DChoiceL *) intros s Qs. destruct (IHderivable s Qs) as (s' & Ps' & DS).
+    exists s'. auto using EDChoiceL.
+  - (* DChoiceR *) intros s Qs. destruct (IHderivable s Qs) as (s' & Ps' & DS).
+    exists s'. auto using EDChoiceR.
+  - (* DIterZero *) intros s Ps. exists s. split. assumption. constructor.
+  - (* DIterNonzero *) intros s Qs. destruct (IHderivable s Qs) as (s' & Ps' & DS).
+    exists s'. auto using star_equiv.
+  - (* DBackwardVariant *)
+    assert (Aux : forall n sig, P n sig ->
+              exists sig', P O sig' /\ [[ c** ]] m |=> (sig', sig)). {
+      induction n; intros sig Pnsig.
+      - exists sig. split. assumption. constructor.
+      - destruct (H0 n sig Pnsig) as (sig' & Pn'sig' & DS).
+        destruct (IHn sig' Pn'sig') as (sig0 & P0 & DStar).
+        exists sig0. split. assumption. econstructor; eassumption.
+    }
+    intros sig (n & Pnsig). destruct (Aux n sig Pnsig) as (sig' & P0 & DStar).
+    exists sig'. auto.
+  - (* DAssume *) intros sig (Psig & Bsig).
+    exists sig. split. assumption. constructor. apply Bsig.
+  - (* DAssign *) intros sig (x' & Psig & Eq).
+    exists (mode_upd m sig x x'). split. assumption.
+    destruct m; unfold mode_store, mode_upd in *; simpl in *.
+      now apply step_assign_ok.
+      now apply step_assign_ad.
+  - (* DRand *) intros sig (x' & Psig).
+    exists (mode_upd m sig x x'). split. assumption.
+    destruct m; unfold mode_upd in *; simpl in *.
+      apply step_rand_ok.
+      apply step_rand_ad.
+  - (* DRead *) intros sig (v & x' & l & Psig & Hl & Hx).
+    exists (mode_chan_upd m (mode_upd m sig x x') s (v :: l)). split. assumption.
+    destruct m; unfold mode_chan_upd, mode_upd, mode_chan, mode_store in *; simpl in *.
+      now apply step_read_ok.
+      now apply step_read_ad.
+  - (* DWrite *) intros sig (l & Psig & Hl).
+    exists (mode_chan_upd m sig s l). split. assumption.
+    destruct m; unfold mode_chan_upd, mode_chan, mode_store in *; simpl in *.
+      now apply step_write_ok.
+      now apply step_write_ad.
+  - (* DAdvAssertSuccess *) intros sig (Qsig & Bsig).
+    exists sig. auto using EDAdvAssertSuccess.
+  - (* DAdvAssertFailure *) intros sig (Qsig & nBsig).
+    exists sig. auto using EDAdvAssertFailure.
+Qed.
